(* New FStar Style VRF code *)

VRF/Spec.VRF.fst
@@ -1,262 +1,135 @@
 module Spec.VRF
 
-open FStar.UInt32
-open FStar.UInt8
-open FStar.Seq
-open FStar.Option
+open Spec.Lib.IntTypes
+open Spec.Lib.IntSeq
+open Spec.Lib.RawIntTypes
 
-open FStar.Mul
-open FStar.Seq
-open FStar.UInt
-
-open FStar.Endianness
 open Spec.Curve25519
 open Spec.Ed25519
-
-open Spec.SHA2_256
-
+open Spec.SHA2
+open FStar.Option
 
 #reset-options "--max_fuel 0 --z3rlimit 100"
 
-let bytes =  seq FStar.UInt8.t
-let key = lbytes 32
-let field = prime
-
 let n = 16
 
+let _OS2ECP (s:lbytes 32) : Tot (option ext_point) =
+	point_decompress s
 
-let d : elem = 37095705934669439343138083508754565189542113879843219016388785533085940283555
-type twisted_edward_point = ext_point
+let _ECP2OS (p:ext_point) : Tot (lbytes 32) = 
+	point_compress p
 
-let g_x : elem = 15112221349535400772501151409588531511454012693041857206046113283949847762202
-let g_y : elem = 46316835694926478169428394003475163141307993866256225615783033603165251855960
+let _I2OSP (value: nat{value < pow2 256}) : Tot (lbytes 32) = 
+	nat_to_bytes_le 32 value	
 
+let _OS2IP (s: lbytes 32) : Tot (elem) = 
+	let n = nat_from_bytes_le #32 s in 
+	n % prime
 
-let cardinality = 57896044618658097711785492504343953926856930875039260848015607506283634007912
+let _OS2IP_16 (s: lbytes 16) : Tot (elem) = 
+	let n = nat_from_bytes_le #16 s in 
+	n % prime
 
-let generator: twisted_edward_point = (g_x, g_y, 1, g_x `fmul` g_y)
+let maxHash = (maxint(U64) + 1)/8
 
-val pointMultiplication : point : twisted_edward_point -> k: bytes -> Tot twisted_edward_point
-let pointMultiplication point k = 
-	Spec.Ed25519.point_mul k point
+let hash (len:size_nat{len < maxHash}) (input:lbytes len)  = 
+	hash256	len input
 
-val scalarAddition : p : twisted_edward_point -> q: twisted_edward_point -> Tot twisted_edward_point
-let scalarAddition p q = 
-	Spec.Ed25519.point_add p q 
+let curveOrder : elem = 7237005577332262213973186563042994240857116359379907606001950938285454250989	
 
-val isPointOnCurve: point : option twisted_edward_point -> Tot bool
-let isPointOnCurve point =
-	if isNone point then false else
-	let point = get point in 
-	let px, py, pz, pt = point in 
-	let x2 = fmul px px in 
-	let y2 = fmul py py in 
-	let left = fsub x2 y2 in 
-	let z2 = fmul pz pz in 
-	let t2 = fmul pt pt in 
-	let dt2 = fmul d t2 in 
-	let right = fadd z2 dt2 in 
-	(left = right)
+val _ECVRF_hash_to_curve: ctr: nat {ctr <= curveOrder} -> pub: lbytes 32 -> len : size_nat{len < maxint U32 - 64} -> 
+	input: (lbytes len) -> Tot (option ext_point)
+	(decreases (curveOrder - ctr))
 
-val _ECP2OS : gamma: twisted_edward_point -> Tot(r: bytes {Seq.length r = 32})
-let _ECP2OS gamma = point_compress gamma
-
-val _OS2ECP : point: bytes{Seq.length point = 32} -> Tot(option twisted_edward_point)
-let _OS2ECP point = point_decompress point
-
-val nat_to_uint8: x: int {x < 256} -> Tot(FStar.UInt8.t)
-let nat_to_uint8 x = FStar.UInt8.uint_to_t (to_uint_t 8 x)
-
-val uint8_to_int : x: FStar.UInt8.t -> Tot(int)
-let uint8_to_int x = FStar.UInt8.v x
-
-val _helper_I2OSP: value: nat -> s: bytes -> counter : nat {counter < Seq.length s} -> 
-		Tot (r: bytes {Seq.length r = Seq.length s})
-		(decreases (counter))
-let rec _helper_I2OSP value s counter  = 
-	let mask = 256 in 
-	let r = value % mask in 
-	let r = nat_to_uint8 r in 
-	let s = upd s counter r in 
-	let number = value / mask  in 
-		if (counter -1 >=0 ) then 
-			_helper_I2OSP number s (counter -1 )
-	else s
-
-val _I2OSP: value: nat -> n: int{n > 0} -> Tot(r: bytes{Seq.length r = n})
-let _I2OSP value n = 
-	if (pow2 (n * 8)  <= value) then Seq.create n 0uy (* changed*)
-	else 
-		let s = Seq.create n 0uy in 
-	(_helper_I2OSP value s (n -1))
-
-val _helper_OS2IP: s: bytes  -> counter: nat {counter < Seq.length s} -> number: nat -> Tot (nat)(decreases (Seq.length s - counter))
-
-let rec _helper_OS2IP s counter number = 
-	let temp = Seq.index s counter in 
-	let temp = uint8_to_int temp in 
-	let counter_mult = pow2 (8 * (Seq.length s - counter -1 )) in 
-	let number = number + (op_Multiply counter_mult temp) in 
-	if (counter +1 < Seq.length s) then  
-		_helper_OS2IP s (counter +1 ) number
-	else 
-		number	
-
-val _OS2IP: s: bytes{Seq.length s > 0} -> nat
-let _OS2IP s = 
-	_helper_OS2IP s 0 0
-
-val seqConcat : s1: seq 'a -> s2: seq 'a -> 
-			Tot(r:seq 'a{Seq.length	r = Seq.length s1 + Seq.length s2})
-
-let seqConcat s1 s2 = 
-	FStar.Seq.append s1 s2 	
-
-val hash: input: bytes{Seq.length input < Spec.SHA2_256.max_input_len_8} -> 
-		Tot(r: bytes{Seq.length r = Spec.SHA2_256.size_hash})	
-let hash input = 
-	Spec.SHA2_256.hash input
-
-
-
-
-val _ECVRF_decode_proof: 
-		pi: bytes {Seq.length pi = op_Multiply 5 n} -> 
-		Tot(
-				tuple3 (option twisted_edward_point)
-		 		(c:bytes{Seq.length c = n})
-		 		(s:bytes {Seq.length s = (op_Multiply 2 n)})
-			)
+let rec  _ECVRF_hash_to_curve ctr pub len input = 
+	let tmp =  create (len + 64) (u8 0) in 
+	let tmp = update_sub #_ #_ tmp 0 len input in 
+	let tmp = update_sub #_ #_ tmp len 32 pub in 
+	let tmp = update_sub #_ #_ tmp (len + 32) 32 (_I2OSP ctr) in 
+	let hashed = hash (len + 64) tmp in 
+	let possiblePoint = _OS2ECP hashed in 
+	match possiblePoint with 
+		| Some p -> Some p
+		| None -> if ctr < curveOrder then 
+				_ECVRF_hash_to_curve (ctr + 1) pub len input
+			else
+				None	
+	
+val _ECVRF_decode_proof: pi: lbytes (op_Multiply n 5) -> Tot 
+	(tuple3 (option ext_point) (lbytes n) (lbytes (op_Multiply 2 n)))
 
 let _ECVRF_decode_proof pi = 
-	let gamma, cs = Seq.split pi (op_Multiply 2 n) in 
-		assert(Seq.length cs =(op_Multiply 3 n));
-	let c, s = Seq.split cs n in 
-		assert(Seq.length s = (op_Multiply 2 n));
-	let point = _OS2ECP gamma in 
-	(point, c, s)
+	let gamma = slice pi 0 (op_Multiply n 2) in 
+	let c = slice pi (op_Multiply n 2) (op_Multiply n 3) in 
+	let s = slice pi (op_Multiply n 3) (op_Multiply n 5) in 
+	(_OS2ECP gamma, c, s)
 
+val _ECVRF_hash_points: g: ext_point -> h: ext_point -> pub: ext_point -> gamma: ext_point -> 
+	gk: ext_point -> hk: ext_point -> Tot elem
 
-val _helper_ECVRF_hash_to_curve : 
-	ctr : nat{ctr < field} ->counter_length:nat{counter_length > 0} ->  
-	pk: bytes{Seq.length pk = 32} ->
-	input: bytes{Seq.length input < Spec.SHA2_256.max_input_len_8 - 32 - counter_length } ->
-	Tot(r: option twisted_edward_point) 
-	(decreases(field - ctr)) 
+let _ECVRF_hash_points g h pub gamma gk hk = 
+	let tmp = create 192 (u8 0) in 
+	let tmp = update_sub #_ #_ tmp 0 32 (_ECP2OS g) in 
+	let tmp = update_sub #_ #_ tmp 32 32 (_ECP2OS h) in 
+	let tmp = update_sub #_ #_ tmp 64 32 (_ECP2OS pub) in 
+	let tmp = update_sub #_ #_ tmp 96 32 (_ECP2OS gamma) in 
+	let tmp = update_sub #_ #_ tmp 128 32 (_ECP2OS gk) in 
+	let tmp = update_sub #_ #_ tmp 160 32 (_ECP2OS hk) in 
+	_OS2IP (hash 192 tmp)
 
-let rec _helper_ECVRF_hash_to_curve ctr counter_length pk input = 
-	let _CTR = _I2OSP ctr counter_length in 
-	let toHash = seqConcat input pk in 
-	let toHash = seqConcat toHash _CTR in 
-	let hash = hash toHash in
-	let possible_point = point_decompress hash in 
-	if isNone possible_point then 
-		(
-			if (ctr + 1) < field then 
-					(_helper_ECVRF_hash_to_curve (ctr+1) counter_length pk input) else
-			None
-		)
-		else 
-			possible_point				
+val _ECVRF_prove: len : size_nat{len < maxint U32 - 64} -> input: (lbytes len) -> pub: lbytes 32 -> priv: lbytes 32 -> k: elem ->
+	Tot (option (lbytes (op_Multiply n 5)))
 
-val _ECVRF_hash_to_curve: input: bytes{Seq.length input < Spec.SHA2_256.max_input_len_8 - 36 } -> 
-			public_key: (twisted_edward_point) -> Tot(option twisted_edward_point)			
+let _ECVRF_prove len input pub priv k = 
+	let ap = point_decompress pub in 
+		if isNone ap then None else
+	let ap = get ap in 
+	let h = _ECVRF_hash_to_curve 0 pub len input in 
+		if isNone h then None else 
+	let h = get h in 	
+	let gamma = point_mul 32 priv h in 
+	let kPrime = _I2OSP k in 
+	let gk = point_mul 32 kPrime g in 
+	let hk = point_mul 32 kPrime h in 
+	let c = _ECVRF_hash_points g h ap gamma gk hk in 
+	let cPrime = fmul c (_OS2IP priv) in 
+	let s = fsub k cPrime in 
+	let tmp = create 80 (u8 0) in 
+	let tmp = update_sub #_ #_ tmp 0 32 (_ECP2OS gamma)	in 
+	let halfC = slice (_I2OSP c) 0 16 in 
+	let tmp = update_sub #_ #_ tmp 32 16 halfC in 
+	let tmp = update_sub #_ #_ tmp 48 32 (_I2OSP s) in 
+	Some tmp
 
-let _ECVRF_hash_to_curve input public_key = 
-	let ctr = 0 in 
-	let pk = _ECP2OS public_key in 
-	let point = _helper_ECVRF_hash_to_curve ctr 4 pk input in point
+val _ECVRF_proof_to_hash: pi: lbytes (op_Multiply n 5 ) -> Tot (option (lbytes (op_Multiply 2 n)))
 
-val _ECVRF_hash_points : generator: twisted_edward_point -> h:  twisted_edward_point -> 
-			public_key: twisted_edward_point -> gamma : twisted_edward_point -> 
-			gk : twisted_edward_point -> hk : twisted_edward_point -> 
-			Tot(nat)
+let _ECVRF_proof_to_hash pi = 
+	let (gamma, c, s ) = _ECVRF_decode_proof pi in 
+	if isNone gamma then None else
+	let gamma = get gamma in 
+	let gammaPrime = _ECP2OS gamma in 
+	let hashed = hash 32 gammaPrime in 
+	Some hashed
 
-let _ECVRF_hash_points generator h public_key gamma gk hk = 
-	let p = _ECP2OS generator in (*32 *)
-	let p = seqConcat p (_ECP2OS h) in (* 64  *)
-	let p = seqConcat p (_ECP2OS public_key) (* 32*3 *) in 
-	let p = seqConcat p (_ECP2OS gamma)  (* still less than 2pow 61 *)in 
-	let p = seqConcat p (_ECP2OS gk) in 
-	let p = seqConcat p (_ECP2OS hk) in 
-	let h' = hash p in 
-	let h = fst (FStar.Seq.split h' n) in 
-	_OS2IP h
-
-val little_endian_ins:	a: bytes -> 
-			counter: nat {counter < Seq.length a} -> 
-			b: bytes{Seq.length a = Seq.length b}-> 
-			Tot (r: bytes{Seq.length a = Seq.length r})
-			(decreases(Seq.length a - counter))
-
-let rec little_endian_ins a counter b = 
-	let element = Seq.index a counter in 
-	let newSeq = Seq.upd b (Seq.length a -1 - counter) element in 
-	if (counter+1 < Seq.length a) then 
-		little_endian_ins a (counter+1) newSeq
-	else 
-		newSeq	
-
-val little_endian_: a: bytes{Seq.length a > 0} -> Tot (r: bytes {Seq.length a = Seq.length r})
-let little_endian_ a = 
-	let s = Seq.create (Seq.length a) 0uy in 
-	little_endian_ins a 0 s
-
-val _ECVRF_prove: input: bytes {Seq.length input < Spec.SHA2_256.max_input_len_8 - 36 } ->  
-			public_key: twisted_edward_point -> 
-			private_key : bytes{Seq.length private_key > 0} ->
-			Tot(proof: option bytes {Some?proof ==> Seq.length (Some?.v proof) = op_Multiply 5 n})
-
-let _ECVRF_prove input public_key private_key = 
-	let h = _ECVRF_hash_to_curve input public_key in 
-		if isNone h then None (* trying to convert the hash to point, if it was not possible returns None *)
-		else 
-			let h = get h in 		
-		let private_keyLE = little_endian_ private_key in 		
-	let gamma = pointMultiplication h private_keyLE in 
-	let k_ = random cardinality in 
-	let k =  _I2OSP k_ 32 in 
-	let kLE = little_endian_ k in 
-		let gk = pointMultiplication generator kLE in  
-		let hk = pointMultiplication h kLE in 
-	let c = _ECVRF_hash_points generator h public_key gamma gk hk in 
-			let cPrivateKey = op_Multiply c (_OS2IP private_key) in  
-			let cPrivateKeyModQ = cPrivateKey % cardinality in 
-	let k_  = k_ + cardinality in 
-	let s = k_ - cPrivateKeyModQ in 
-	let s = s % cardinality in 
-			let fst = _ECP2OS gamma in 
-			let snd = _I2OSP c n in (* Seq length snd = n*)
-			let thd = _I2OSP s (op_Multiply 2 n) (* Seq.length thr = 2n *) in 
-	let pi = seqConcat fst (seqConcat snd thd) in Some pi
-
-val _ECVRF_proof2hash: pi: bytes{Seq.length pi = op_Multiply 5 n } -> Tot(hash: bytes{Seq.length hash = n})
-
-let _ECVRF_proof2hash pi = 
-	let right_part = snd( Seq.split pi (op_Multiply 2 n)) in 
-	fst (Seq.split right_part n)
-
-val _ECVRF_verify :
-		public_key : twisted_edward_point ->
-		proof: bytes {Seq.length proof = op_Multiply 5 n } -> 
-		input : bytes{Seq.length input < Spec.SHA2_256.max_input_len_8 - 36 } -> 
-		Tot(bool)
-
-let _ECVRF_verify public_key proof input = 
-	let gamma, c, s = _ECVRF_decode_proof proof in 
-	if isNone gamma then false
-		else let gamma = get gamma in 
-	let cLE = little_endian_ c in 
-	let sLE = little_endian_ s in 	
-	let yc = pointMultiplication public_key cLE in 
-	let gs = pointMultiplication generator sLE in 
-	let u  = scalarAddition yc gs in 
-	let h = _ECVRF_hash_to_curve input public_key in 
-		if isNone h then false
-	else 
+val _ECVRF_verify:  len : size_nat{len < maxint U32 - 64} -> input: (lbytes len) -> pub: lbytes 32 ->
+	pi: lbytes (op_Multiply n 5 ) ->Tot bool
+	
+let _ECVRF_verify len input pub pi = 
+	let ap = point_decompress pub in 
+		if isNone ap then false else
+	let ap = get ap in 
+	let (gamma, c, s ) = _ECVRF_decode_proof pi in 
+		if isNone gamma then false else
+	let gamma = get gamma in 
+	let yc = point_mul 16 c ap in 
+	let gs = point_mul 32 s g in 
+	let u = point_add yc gs in 
+	let h = _ECVRF_hash_to_curve 0 pub len input in 
+		if isNone h then false else 
 	let h = get h in 
-	let gammac = pointMultiplication gamma cLE in 
-	let hs = pointMultiplication h sLE in 
-	let v = scalarAddition gammac hs in 
-	let c_prime = _ECVRF_hash_points generator h public_key gamma u v in 
-	(_OS2IP c) = c_prime
+	let gammac = point_mul 16 c gamma in 
+	let hs = point_mul 32 s h in 
+	let v = point_add gammac hs in 
+	let c_prime = _ECVRF_hash_points g h ap gamma u v in 
+	c_prime % pow2 128 = _OS2IP_16 c
+
